Logic/FoundationPort/Coq/Audit.v
@@ -332,7 +332,10 @@ Check semiformula_bex_mem.
 Check first_order_structure.
 Check unit_first_order_structure.
 Check first_order_structure_language_map.
+Check carrier_equiv.
+Check first_order_structure_transport.
 Check fin_env_cons.
+Check carrier_equiv_from_fin_env_cons.
 Check semiterm_val.
 Check closed_semiterm_val.
 Check semiterm_val_rewrite.
@@ -343,6 +346,7 @@ Check semiterm_val_map.
 Check semiterm_val_bshift.
 Check semiterm_val_emb_substs.
 Check semiterm_val_language_map.
+Check semiterm_val_transport.
 Check semiterm_val_free_ext.
 Check semiformula_eval.
 Check formula_eval.
@@ -360,16 +364,19 @@ Check semiformula_eval_bshift.
 Check semiformula_eval_emb_substs.
 Check semiformula_eval_free_ext.
 Check semiformula_eval_language_map.
+Check semiformula_eval_transport.
 Check semiterm_operator_val.
 Check semiterm_val_operator_apply.
 Check semiterm_operator_val_comp.
 Check semiterm_operator_val_bvar.
 Check semiterm_operator_val_fn.
+Check semiterm_operator_val_transport.
 Check semiformula_operator_eval.
 Check semiformula_eval_operator_apply.
 Check semiformula_operator_eval_comp.
 Check semiformula_operator_eval_and.
 Check semiformula_operator_eval_or.
+Check semiformula_operator_eval_transport.
 Check semiformula_eq_operator_eval_of_language.
 Check semiformula_lt_operator_eval_of_language.
 Check semiformula_mem_operator_eval_of_language.
@@ -384,6 +391,7 @@ Check structure_interprets_lt.
 Check structure_interprets_le.
 Check structure_interprets_mem.
 Check structure_interprets_le_of_eq_lt.
+Check structure_interprets_le_of_eq_lt_spec.
 Check semiterm_val_binary_bound.
 Check semiformula_eval_bounded_operator_all.
 Check semiformula_eval_bounded_operator_exists.
@@ -508,17 +516,22 @@ Print Assumptions semiformula_eq_operator_injective.
 Print Assumptions semiformula_le_operator_injective.
 Print Assumptions semiterm_val_rewrite.
 Print Assumptions semiterm_val_language_map.
+Print Assumptions semiterm_val_transport.
 Print Assumptions semiterm_val_free_ext.
 Print Assumptions semiformula_eval_neg.
 Print Assumptions semiformula_eval_bounded_all.
 Print Assumptions semiformula_eval_rewrite.
 Print Assumptions semiformula_eval_free_ext.
 Print Assumptions semiformula_eval_language_map.
+Print Assumptions semiformula_eval_transport.
 Print Assumptions semiterm_val_operator_apply.
 Print Assumptions semiterm_operator_val_comp.
+Print Assumptions semiterm_operator_val_transport.
 Print Assumptions semiformula_eval_operator_apply.
 Print Assumptions semiformula_operator_eval_comp.
+Print Assumptions semiformula_operator_eval_transport.
 Print Assumptions structure_interprets_le_of_eq_lt.
+Print Assumptions structure_interprets_le_of_eq_lt_spec.
 Print Assumptions semiformula_eval_bounded_operator_all.
 Print Assumptions semiformula_eval_bounded_operator_exists.
 Print Assumptions semiformula_eval_ball_relation.
